wip

compiler/entry/jasmin2ec.ml
@@ -35,10 +35,11 @@ let parse_and_extract arch call_conv idirs =
     let fresh_var_ident k ii n ty =
       Conv.fresh_var_ident k ii (Uint63.of_int 0) n ty
     in
+    let rename = LegalizeNames.build_rename prog in
     let prog =
       match
         Conv.cuprog_of_prog prog
-        |> ToEC_jazz.toEC_prog A.asm_e fresh_var_ident (model = Normal)
+        |> ToEC_jazz.toEC_prog A.asm_e fresh_var_ident rename (model = Normal)
       with
       | Utils0.Error e ->
           let e = Conv.error_of_cerror (Printer.pp_err ~debug:false) e in
