compiler/src/legalizeNames.mli
@@ -1,0 +1,3 @@
+val build_rename :
+  (unit, 'asm) Prog.prog ->
+  Prog.funname -> Var0.Var.var -> Ident.Ident.ident
