proofs/toEC/init_local_arrays_proof.v
@@ -1,0 +1,149 @@
+From mathcomp Require Import ssreflect ssrfun ssrbool eqtype.
+Require Import psem compiler_util.
+Require Export init_local_arrays.
+
+Section INIT_LOCAL_ARRAYS_PROOF.
+
+Context
+  {wsw : WithSubWord}
+  {dc : DirectCall}
+  {asm_op syscall_state : Type}
+  {ep : EstateParams syscall_state}
+  {spp : SemPexprParams}
+  {sip : SemInstrParams asm_op syscall_state}
+  {E E0 : Type -> Type}
+  {wE : with_Error E E0}
+  {rE0 : EventRels E0}
+.
+
+#[local] Existing Instance progUnit.
+#[local] Existing Instance sCP_unit.
+
+Context
+  (p p' : uprog)
+  (ev : extra_val_t)
+  (init_local_arrays_ok : init_local_arrays_prog p = p')
+.
+
+Lemma init_local_arrays_eq_globs : p_globs p = p_globs p'.
+Proof using init_local_arrays_ok.
+  by move: init_local_arrays_ok; rewrite /init_local_arrays_prog => <-.
+Qed.
+
+Lemma get_fundef_init_local_arrays fn :
+  get_fundef (p_funcs (init_local_arrays_prog p)) fn =
+    omap init_local_arrays_fd (get_fundef (p_funcs p) fn).
+Proof.
+rewrite /get_fundef /init_local_arrays_prog /=.
+by elim: (p_funcs p) => [ | [fn' fd'] pfuns ih] //=; case: eqP.
+Qed.
+
+Lemma vrvs_map_Lvar (xs : seq var_i) :
+  Sv.Equal (vrvs [seq Lvar i | i <- xs]) (vars_l xs).
+Proof using E E0 dc ep rE0 spp syscall_state wE wsw.
+elim: xs => [ | x xs ih] /=; first by SvD.fsetdec.
+by rewrite vrvs_cons vrv_var ih; SvD.fsetdec.
+Qed.
+
+Lemma local_arraysP fd x :
+  x \in local_arrays fd ->
+  is_local_array_var x /\ ~ Sv.In x (vars_l (f_params fd)).
+Proof.
+rewrite /local_arrays mem_filter => /andP [] harr /Sv_elemsP hin.
+split=> //.
+by move: hin; rewrite Sv.diff_spec => -[_].
+Qed.
+
+Lemma init_local_arrays_init_locals fd fs s :
+  initialize_funcall p ev fd fs = ok s ->
+  forall x, x \in local_arrays fd -> (evm s).[x] = Vm.init.[x].
+Proof using E E0 asm_op dc ep ev p rE0 sip spp syscall_state wE wsw.
+rewrite /initialize_funcall; t_xrbindP => vs hargs s0 hini hw x hx.
+have [_ hnotin] := local_arraysP hx.
+move: hw; rewrite (write_vars_lvals _ (p_globs p)) => hw.
+rewrite -(disjoint_eq_ons (s := Sv.singleton x) _ hw).
+- by move: hini => [<-] /=; rewrite Vm.initP.
+- rewrite /disjoint; apply/Sv.is_empty_spec; rewrite vrvs_map_Lvar.
+  by SvD.fsetdec.
+by SvD.fsetdec.
+Qed.
+
+Lemma init_local_array_instrP (ii : instr_info) x s1 s2 :
+  is_local_array_var x ->
+  (evm s1).[x] = Vm.init.[x] ->
+  st_eq tt s1 s2 ->
+  exists2 s2',
+    sem_assgn p' (Lvar {| v_var := x; v_info := dummy_var_info |})
+      AT_none (vtype x)
+      (match vtype x with
+       | aarr ws n => Parr_init ws n
+       | _ => Parr_init U8 0
+       end) s2 = ok s2'
+    & st_eq tt s1 s2'.
+Proof.
+move=> harr hx [hscs hmem hvm].
+move: harr; rewrite /is_local_array_var.
+case hty: (vtype x) => [ | | ws n | ] // _.
+rewrite /sem_assgn /=.
+rewrite /truncate_val /= WArray.castK /=.
+eexists.
+- apply/write_varP; split=> //; rewrite hty /= eqxx //.
+split=> //=.
+move: hvm; rewrite !vm_eq_vm_rel => hu1.
+apply: (vm_rel_set_r (P := PredT)) => //.
+move=> _ /=.
+rewrite hty /=.
+by rewrite if_same hx Vm.initP hty.
+by apply: (vm_relI _ hu1).
+Qed.
+
+Let Rprefix (xs : seq var) (s1 s2 : estate) : Prop :=
+  st_eq tt s1 s2 /\
+  forall x, x \in xs -> is_local_array_var x /\ (evm s1).[x] = Vm.init.[x].
+
+Lemma init_local_arrays_prefixP ii (xs : seq var) :
+  wequiv_rec p p' ev ev eq_spec (Rprefix xs)
+    [::] (map (init_local_array_instr ii) xs) (st_eq tt).
+Proof.
+elim: xs => [ | x xs ih] /=.
+- apply wequiv_nil.
+  by move=> s1 s2 [].
+apply (wequiv_cat (R := Rprefix xs)
+  (c1 := [::]) (c1' := [::])
+  (c2 := [:: init_local_array_instr ii x])
+  (c2' := map (init_local_array_instr ii) xs)).
+- apply wequiv_assign_right => s1 s2 [heq hloc].
+  have [harr hx] := hloc x (mem_head _ _).
+  have [s2' heq1 heq2] := init_local_array_instrP ii harr hx heq.
+  exists s2'; first exact: heq1.
+  split=> //.
+  by move=> y hy; apply: hloc; rewrite in_cons hy orbT.
+exact: ih.
+Qed.
+
+Lemma init_local_arrays_proof fn :
+  wiequiv_f p p' ev ev (rpreF (eS := eq_spec)) fn fn (rpostF (eS := eq_spec)).
+Proof using init_local_arrays_ok.
+apply wequiv_fun_ind => {}fn _ fs _ [<- <-] fd hget.
+exists (init_local_arrays_fd fd).
+- by rewrite -init_local_arrays_ok get_fundef_init_local_arrays hget.
+move=> s11 hinit.
+exists s11.
+- by apply: (eq_initialize _ _ _ _ hinit) => //; rewrite -init_local_arrays_ok.
+exists (Rprefix (local_arrays fd)), (st_eq tt); split.
+- split=> //.
+  move=> x hx; split; [case: (local_arraysP hx) => // |
+    exact (init_local_arrays_init_locals hinit hx)].
+- rewrite /init_local_arrays_fd /init_local_arrays_body /=.
+  rewrite -{1}(cat0s (f_body fd)).
+  apply (wequiv_cat (R := st_eq tt)
+    (c1 := [::]) (c1' := f_body fd)
+    (c2 := map (init_local_array_instr (entry_info_of_fun_info (f_info fd)))
+             (local_arrays fd))
+    (c2' := f_body fd)).
+  + exact: init_local_arrays_prefixP.
+  by apply/wequiv_rec_st_eq/init_local_arrays_eq_globs.
+exact: (st_eq_finalize erefl erefl erefl).
+Qed.
+
+End INIT_LOCAL_ARRAYS_PROOF.
