proofs/toEC/remove_nullary_opns.v
@@ -1,0 +1,63 @@
+Require Import expr.
+
+Section REMOVE_NULLARY_OPNS.
+
+Context
+  {asm_op : Type}
+  {asmop : asmOp asm_op}
+.
+
+#[local] Existing Instance progUnit.
+
+Section CMD.
+
+Context (remove_nullary_opns_i : instr -> cmd).
+
+Fixpoint remove_nullary_opns_c (c : cmd) : cmd :=
+  match c with
+  | [::] => [::]
+  | i :: c => remove_nullary_opns_i i ++ remove_nullary_opns_c c
+  end.
+
+End CMD.
+
+Fixpoint remove_nullary_opns_i (i : instr) : cmd :=
+  let 'MkI ii ir := i in
+  match ir with
+  | Cassgn _ _ _ _ | Csyscall _ _ _ | Cassert _ | Ccall _ _ _ => [:: i]
+  | Copn xs t o es => match xs with [::] => [::] | _ => [:: i] end
+  | Cif e c1 c2 =>
+      [:: MkI ii (Cif e (remove_nullary_opns_c remove_nullary_opns_i c1)
+                    (remove_nullary_opns_c remove_nullary_opns_i c2))]
+  | Cfor x r c =>
+      [:: MkI ii (Cfor x r (remove_nullary_opns_c remove_nullary_opns_i c))]
+  | Cwhile al c1 e info c2 =>
+      [:: MkI ii
+            (Cwhile al (remove_nullary_opns_c remove_nullary_opns_i c1) e info
+               (remove_nullary_opns_c remove_nullary_opns_i c2))]
+  end.
+
+Definition remove_nullary_opns_fd (fd : _fundef unit) : _fundef unit :=
+  {|
+    f_info := f_info fd;
+    f_contract := f_contract fd;
+    f_tyin := f_tyin fd;
+    f_params := f_params fd;
+    f_body := remove_nullary_opns_c remove_nullary_opns_i fd.(f_body);
+    f_tyout := f_tyout fd;
+    f_res := f_res fd;
+    f_extra := f_extra fd;
+  |}.
+
+Definition remove_nullary_opns_fun_decl
+  (fd : funname * _fundef unit) : funname * _fundef unit :=
+  let '(fn, fd) := fd in (fn, remove_nullary_opns_fd fd).
+
+Definition remove_nullary_opns_prog (p : _uprog) : _uprog :=
+  {|
+    p_funcs := map remove_nullary_opns_fun_decl (p_funcs p);
+    p_globs := p_globs p;
+    p_extra := p_extra p;
+  |}.
+
+End REMOVE_NULLARY_OPNS.
